crypto_examples/bins.dfy
@@ -5,4 +5,21 @@ module bins refines LittleEndianNat {
     {
         2
     }
+
+    lemma BitSelModEquivalence(a: seq<uint>, i: nat)
+        requires 0 <= i < |a|;
+        ensures Pow(2, i) > 0;
+        ensures IsModEquivalent(a[i], ToNatRight(a) / Pow(2, i), 2);
+        ensures a[i] == (ToNatRight(a) / Pow(2, i)) % 2;
+    {
+        LemmaSeqPrefix(a, i);
+        assert ToNatRight(a[..i]) + ToNatRight(a[i..]) * Pow(2, i) == ToNatRight(a);
+        LemmaSeqNatBound(a[..i]);
+        // LemmaPowStrictlyIncreasesAuto();
+        assert ToNatRight(a[..i]) < Pow(2, i);
+        LemmaFundamentalDivModConverse(ToNatRight(a), Pow(2, i), ToNatRight(a[i..]), ToNatRight(a[..i]));
+
+        assert ToNatRight(a) / Pow(2, i) == ToNatRight(a[i..]);
+        LemmaSeqLswModEquivalence(a[i..]);
+    }
 }
